---
{"dg-publish":true,"permalink":"/world/summa-kvadratov/"}
---

#math #series
## Сумма
$1^{2}+2^{2}+\dots+n^{2} = \frac{n(n+1)(2n+1)}{6}$

## Вывод
$(a+b)^{3}= a^{3} + 3a^{2}b + 3ab^{2} + b^{3}$
$(a+1)^{3}= a^{3} + 3a^{2} + 3a + 1$

$(1+1)^{3} = 1^{3} + 3*1^{2} + 3*1 + 1 = 2^{3}$
$(2+1)^{3} = 2^{3} + 3*2^{2} + 3*2 + 1 = 3^{3}$
$\dots$
$(n+1)^{3} = n^{3} + 3*n^{2} + 3*n + 1$

$2^{3} + 3^{3} + \dots + (n+1)^{3} = (1^{3} + 2^{3} + \dots + n^{3}) + 3(1^{2}+2^{2}+\dots+n^{2}) + 3(1+2+\dots+n) + n =$
$(n+1)^{3} = 1 + 3(1^{2}+2^{2}+\dots+n^{2}) + 3n\frac{n+1}{2} + n$
$1^{2}+2^{2}+\dots+n^{2} = \frac{(n+1)^{3} - 3n\frac{n+1}{2} - (n+1)}{3} = (n+1) \frac{(n+1)^{2} - \frac{3n}{2} - 1}{3} = (n+1) \frac{n^{2} +2n + 1 - \frac{3n}{2} - 1}{3} = (n+1) \frac{2n^{2} + 4n - 3n}{6} =$
$\frac{n(n+1)2n + 1}{6}$
